Hs.lean
@@ -1,3 +1,5 @@
 import Hs.HsTerm
 import Hs.HsJudgment
+import Hs.Algorithm
 import Hs.Compile
+import Hs.Metatheory.Preservation
