Hs/Algorithm/Soundness.lean
@@ -1,0 +1,28 @@
+import Hs.HsTerm
+import Hs.Algorithm
+import Hs.HsJudgment
+import Hs.Compile
+
+set_option maxHeartbeats 500000
+
+theorem compile_soudness :
+  (j : Γ ⊢s t : τ) ->
+  compile Γ t τ j = .some t' ->
+  CompileJ .term Γ ⟨t, τ; j, t'⟩ := by
+intro j c;
+unfold compile at c; split at c;
+case _ => sorry
+case _ => sorry
+case _ => sorry
+case _ => sorry
+case _ => sorry
+case _ => sorry
+case _ => sorry
+case _ => sorry
+case _ => sorry
+case _ => sorry
+case _ => sorry
+case _ => sorry
+case _ => sorry
+case _ => sorry
+case _ => sorry
