Hs/Metatheory/FrameWf.lean
@@ -1,0 +1,234 @@
+import Hs.HsTerm
+import Hs.HsJudgment
+import SystemFD.Ctx
+import Hs.Metatheory.Weaken
+import Hs.Metatheory.TypeMatch
+
+namespace FrameWf
+  def weaken (r : Ren) :
+    ⊢s Δ ->
+    (∀ x, (Γ d@ x).apply r.to = Δ d@ (r x)) ->
+    Γ ⊢s f ->
+    Δ ⊢s f.apply r.to
+  := by
+  intro wf h j
+  cases j
+  case _ =>
+    unfold Frame.apply; simp; constructor
+    apply wf
+  case _ j =>
+    unfold Frame.apply; simp; constructor
+    have lem := rename r .prf j wf h; simp at lem
+    apply lem
+  case _ j =>
+    unfold Frame.apply; simp; constructor
+    have lem := rename r .prf j wf h; simp at lem
+    apply lem
+  case _ j =>
+    unfold Frame.apply; simp; constructor
+    have lem := rename r .prf j wf h; simp at lem
+    apply lem
+  case _ j1 j2 =>
+    unfold Frame.apply; simp; constructor
+    have lem := rename r .prf j1 wf h; simp at lem
+    apply lem; apply valid_ctor_subst _ _ j2
+    case _ =>
+      intro n y h2; rw [h]
+      unfold Ren.to at h2; simp at h2; subst h2
+      simp
+    case _ =>
+      intro n h2; unfold Ren.to; simp
+  -- case _ j =>
+  --   unfold Frame.apply; simp; constructor
+  --   have lem := rename r .prf j wf h; simp at lem
+  --   apply lem
+  -- case _ j =>
+  --   unfold Frame.apply; simp; constructor
+  --   have lem := rename r j wf h; simp at lem
+  --   apply lem
+  -- case _ j1 j2 =>
+  --   unfold Frame.apply; simp; constructor
+  --   have lem := rename r j1 wf h; simp at lem
+  --   apply lem; apply valid_insttype_subst _ _ j2
+  --   case _ =>
+  --     intro n y h2; rw [h]
+  --     unfold Ren.to at h2; simp at h2; subst h2
+  --     simp
+  --   case _ =>
+  --     intro n h2; unfold Ren.to; simp
+  -- case _ x T t j1 j2 =>
+  --   have h2 := h x; rw [<-j1] at h2
+  --   unfold Frame.apply at h2; simp at h2
+  --   constructor; apply h2
+  --   have lem := rename r j2 wf h; simp at lem
+  --   apply lem
+  case _ j1 j2 =>
+    unfold Frame.apply; simp; constructor
+    have lem1 := rename r .prf j1 wf h; simp at lem1; apply lem1
+    have lem2 := rename r .prf j2 wf h; simp at lem2; apply lem2
+end FrameWf
+
+-- @[simp]
+-- abbrev FrameWfByIndexLemmaType (Γ : Ctx HsTerm) : (v : JudgmentVariant) -> HsJudgmentArgs v -> Type
+-- | .prf => λ _ => Int
+-- | .wf => λ () => ∀ x, Γ ⊢s Γ d@ x
+
+def hs_frame_wf_by_index_lemma : (v : JudgmentVariant) -> (ix : HsJudgmentArgs v)
+  -> HsJudgment v Γ ix
+  -> ∀ x, Γ ⊢s Γ d@ x
+:= sorry
+
+
+-- by
+-- intro j; induction j <;> simp at *
+-- case _ => constructor; constructor
+-- case _ wf ih =>
+--   intro x; cases x <;> simp at *
+--   case _ =>
+--     unfold Frame.apply; simp; constructor
+--     constructor; apply wf
+--   case _ x =>
+--     apply FrameWf.weaken (· + 1) _ _ (ih x)
+--     constructor; apply wf
+--     case _ =>
+--       intro y; simp; unfold S; unfold Ren.to
+--       simp
+-- case _ j1 j2 ih1 ih2 =>
+--   intro x; cases x <;> simp at *
+--   case _ =>
+--     unfold Frame.apply; simp; constructor
+--     have lem := weaken_type j1 j1; simp at lem
+--     apply lem;
+--   case _ x =>
+--     apply FrameWf.weaken (· + 1) _ _ (ih2 x)
+--     case _ => apply HsJudgment.wftype j1 j2
+--     case _ =>
+--       intro y; simp; unfold S; unfold Ren.to
+--       simp
+-- case _ j1 j2 ih1 ih2 =>
+--   intro x; cases x <;> simp at *
+--   case _ =>
+--     unfold Frame.apply; simp; constructor
+--     have lem := weaken_kind j1 j1; simp at lem
+--     apply lem;
+--   case _ x =>
+--     apply FrameWf.weaken (· + 1) _ _ (ih2 x)
+--     case _ => apply HsJudgment.wfkind j1 j2
+--     case _ =>
+--       intro y; simp; unfold S; unfold Ren.to
+--       simp
+-- case _ j1 j2 ih1 ih2 =>
+--   intro x; cases x <;> simp at *
+--   case _ =>
+--     unfold Frame.apply; simp; constructor
+--     have lem := weaken_datatype j1 j1; simp at lem
+--     apply lem;
+--   case _ x =>
+--     apply FrameWf.weaken (· + 1) _ _ (ih2 x)
+--     case _ => apply HsJudgment.wfdatatype j1 j2
+--     case _ =>
+--       intro y; simp; unfold S; unfold Ren.to
+--       simp
+-- case _ j1 j2 j3 ih1 ih2 =>
+--   intro x; cases x <;> simp at *
+--   case _ =>
+--     unfold Frame.apply; simp; constructor
+--     have lem := weaken_ctor j1 j3 j1; simp at lem
+--     apply lem; apply valid_ctor_subst _ _ j3
+--     case _ =>
+--       intro n y h; unfold S at h
+--       injection h with e; subst e; simp
+--     case _ =>
+--       intro n h; exists n + 1
+--   case _ x =>
+--     apply FrameWf.weaken (· + 1) _ _ (ih2 x)
+--     case _ => apply HsJudgment.wfctor j1 j2 j3
+--     case _ =>
+--       intro y; simp; unfold S; unfold Ren.to
+--       simp
+-- -- case _ j1 j2 ih1 ih2 =>
+-- --   intro x; cases x <;> simp at *
+-- --   case _ =>
+-- --     unfold Frame.apply; simp; constructor
+-- --     have lem := weaken_opent j1 j1; simp at lem
+-- --     apply lem;
+-- --   case _ x =>
+-- --     apply FrameWf.weaken (· + 1) _ _ (ih2 x)
+-- --     case _ => apply HsJudgment.wfopent j1 j2
+-- --     case _ =>
+-- --       intro y; simp; unfold S; unfold Ren.to
+-- --       simp
+-- -- case _ j1 j2 ih1 ih2 =>
+-- --   intro x; cases x <;> simp at *
+-- --   case _ =>
+-- --     unfold Frame.apply; simp; constructor
+-- --     have lem := weaken_openm j1 j1; simp at lem
+-- --     apply lem;
+-- --   case _ x =>
+-- --     apply FrameWf.weaken (· + 1) _ _ (ih2 x)
+-- --     case _ => apply Judgment.wfopenm j1 j2
+-- --     case _ =>
+-- --       intro y; simp; unfold S; unfold Ren.to
+-- --       simp
+-- -- case _ j1 j2 j3 ih1 ih2 =>
+-- --   intro x; cases x <;> simp at *
+-- --   case _ =>
+-- --     unfold Frame.apply; simp; constructor
+-- --     have lem := weaken_insttype j1 j3 j1; simp at lem
+-- --     apply lem; apply valid_insttype_subst _ _ j3
+-- --     case _ =>
+-- --       intro n y h; unfold S at h
+-- --       injection h with e; subst e; simp
+-- --     case _ =>
+-- --       intro n h; exists n + 1
+-- --   case _ x =>
+-- --     apply FrameWf.weaken (· + 1) _ _ (ih2 x)
+-- --     case _ => apply Judgment.wfinsttype j1 j2 j3
+-- --     case _ =>
+-- --       intro y; simp; unfold S; unfold Ren.to
+-- --       simp
+-- -- case _ Γ x T t j1 j2 j3 ih1 ih2 =>
+-- --   have lem1 : .openm ([S]T) = (Γ d@ x).apply S := by
+-- --     rw [<-j1]; unfold Frame.apply; simp
+-- --   intro x; cases x <;> simp at *
+-- --   case _ =>
+-- --     have lem2 := weaken_inst j1 j2 j2; simp at lem2
+-- --     unfold Frame.apply; simp; constructor
+-- --     simp; apply lem1; apply lem2
+-- --   case _ x =>
+-- --     apply FrameWf.weaken (· + 1) _ _ (ih2 x)
+-- --     case _ => apply Judgment.wfinst j1 j2 j3
+-- --     case _ =>
+-- --       intro y; simp; unfold S; unfold Ren.to
+-- --       simp
+-- case _ j1 j2 j3 ih1 ih2 ih3 =>
+--   intro x; cases x <;> simp at *
+--   case _ =>
+--     have lem1 := weaken_term j1 j2 j1; simp at lem1
+--     have lem2 := weaken_term j1 j2 j2; simp at lem2
+--     unfold Frame.apply; simp; constructor
+--     apply lem1; apply lem2
+--   case _ x =>
+--     apply FrameWf.weaken (· + 1) _ _ (ih3 x)
+--     case _ => apply HsJudgment.wfterm j1 j2 j3
+--     case _ =>
+--       intro y; simp; unfold S; unfold Ren.to
+--       simp
+
+def hs_frame_wf_by_index x : ⊢s Γ -> Γ ⊢s Γ d@ x :=
+λ wf => hs_frame_wf_by_index_lemma .wf () wf x
+
+def hs_frame_wf_implies_wf : Γ ⊢s f -> ⊢s Γ
+| .empty h1 => h1
+| .kind h1 => hs_judgment_ctx_wf .prf h1
+| .type h1 => hs_judgment_ctx_wf .prf h1
+| .datatype h1 => hs_judgment_ctx_wf .prf h1
+| .ctor h1 _ => hs_judgment_ctx_wf .prf h1
+| .term h1 _ => hs_judgment_ctx_wf .prf h1
+
+
+def hs_frame_wf_implies_typed_var T :
+  Γ ⊢s Γ d@ x ->
+  .some T = (Γ d@ x).get_type ->
+  Γ ⊢s (.HsVar x) : T :=
+λ fwf gt => HsJudgment.var (hs_frame_wf_implies_wf fwf) gt
