Hs/Metatheory/Preservation.lean
@@ -1,0 +1,91 @@
+import Hs.Compile
+
+
+@[simp]
+abbrev CompileCtxWfType : (v : CompileVariant) -> (Γ : Ctx HsTerm) -> (CompileJArgs v Γ) -> Prop
+| .term => λ Γ => λ ⟨τ , k ; j, τ'⟩ => ∀ Γ',
+  (k = `★) ->  CompileJ .term Γ ⟨τ, k ; j, τ'⟩ -> CompileJ .ctx Γ Γ' ->  Γ' ⊢ τ' : ★
+  -- ∨ (k = `□ ->  Compile .term Γ (⟨τ, k ; j⟩, τ') ->  Compile .ctx Γ Γ' ->  Γ' ⊢ τ' : □)
+| .ctx => λ Γ => λ Γ' => ⊢s Γ -> CompileJ .ctx Γ Γ' -> ⊢ Γ'
+
+theorem compile_wf_ctx :
+ CompileJ v Γ idx -> CompileCtxWfType v Γ idx := by sorry
+-- by
+-- intro j; induction j <;> simp at *;
+-- case _ =>intros; apply Judgment.wfnil;
+-- all_goals (intro j c; cases j; cases c)
+-- case _ ih wf c =>
+--   apply Judgment.wfempty (ih wf c)
+-- case _ ih _ wf _ _ c1 c =>
+--   apply Judgment.wfkind;
+--   sorry;
+--   apply (ih wf c);
+-- case _ Γ' _ _ _ _ _ c ih1 ih2 wf h1 _ h2 c1 c2 =>
+--   simp at Γ';
+--   apply Judgment.wftype;
+--   replace ih1 := ih1 wf c2;
+--   apply ih2 Γ' c; assumption;
+--   apply ih1; assumption; assumption;
+-- case _ Γ' _ _ _ _ _ _ h1' ih1 ih2 wf h1 h2 _ c1 c2 =>
+--   simp at Γ'; apply Judgment.wfterm;
+--   have ih2' := ih2 Γ' sorry h1' c2; assumption;
+--   sorry
+--   apply ih1 wf c2
+-- case _ => sorry
+-- case _ => sorry
+-- case _ => sorry
+-- case _ => sorry
+
+
+theorem compile_type_preserving_index :
+  CompileJ .ctx Γ Γ' ->
+  (Γ d@ x).get_type = .some τ ->
+  CompileJ .term Γ ⟨τ, k; j, τ'⟩ ->
+  (Γ' d@ x).get_type = .some τ' := by
+intro cc gt cτ;
+induction x;
+case _ => sorry
+case _ => sorry
+
+@[simp]
+abbrev CompileTypePreservingType : (v : CompileVariant) -> (Γ : Ctx HsTerm) -> CompileJArgs v Γ -> Prop
+| .term => λ Γ => λ ⟨t, τ ; j, t'⟩ => ∀ Γ' τ',
+  ⊢s Γ ->
+  CompileJ .ctx Γ Γ' ->
+  ⊢ Γ' ->
+  (jτ : Γ ⊢s τ : `★) ->
+  CompileJ .term Γ ⟨τ, `★ ; jτ, τ'⟩ ->
+  CompileJ .term Γ ⟨t, τ ; j, t'⟩ ->
+  Γ' ⊢ t' : τ'
+| .ctx => λ _ => λ _ => true
+
+theorem compile_type_preserving :
+  CompileJ v Γ idx ->
+  CompileTypePreservingType v Γ idx
+ := by sorry
+-- intro j; induction j <;> simp at *;
+-- all_goals (intro Γ' τ' wf cc wf' jτ c1 c2)
+-- case _ => sorry
+-- case _ j1 j2 j3 ck1 ck2 ih1 ih2 => cases c1
+-- case _ j1 c1 j2 j3 j4 c2 ih1 ih2 ih3 => -- bogus case
+--   sorry
+-- case _ =>
+--   cases c2; case _ gt =>
+--   have h := compile_type_preserving_index cc gt c1;
+--   apply Judgment.var wf' (Eq.symm h)
+
+-- theorem compile_valid_ctor_preserving :
+--   (j : Γ ⊢s A : `★) ->
+--   Compile A j A' ->
+--   CompileCtx Γ Γ' ->
+--   ValidHsCtorType Γ A ->
+--   ValidCtorType Γ' A' := by
+-- intro j c1 c2 h;
+-- induction h;
+-- case _ => sorry
+-- case _ j' ih =>
+--   have lem := compile_kind_preserving1 j
+--   replace ih := ih j';
+--   sorry
+-- case _ => sorry
+-- case _ => sorry
