Hs/Metatheory/Weaken.lean
@@ -1,0 +1,174 @@
+import Hs.HsTerm
+import Hs.HsJudgment
+import SystemFD.Ctx
+import Hs.Metatheory.TypeMatch
+
+theorem rename_lift r (A : Frame HsTerm) :
+  (∀ x, (Γ d@ x).apply r.to = Δ d@ (r x)) ->
+  ∀ x, ((A::Γ) d@ x).apply r.lift.to = (A.apply r.to::Δ) d@ (Ren.lift r x)
+:= by
+intro h x; simp
+cases x <;> simp at *
+case _ =>
+  rw [Subst.lift_lemma]; simp
+  unfold Ren.lift; simp
+  rw [Frame.apply_compose, Frame.apply_compose]; simp
+case _ x =>
+  rw [Subst.lift_lemma]; simp
+  unfold Ren.lift; simp
+  rw [<-h x, Frame.apply_compose, Frame.apply_compose]; simp
+
+@[simp]
+abbrev idx_ren (r : Ren) : HsJudgmentArgs v -> HsJudgmentArgs v :=
+  match v with
+  | .prf => λ (t, A) => ([r.to]t, [r.to]A)
+  | .wf => λ () => ()
+
+def rename (r : Ren) : (v : JudgmentVariant) -> {idx : HsJudgmentArgs v} ->
+  HsJudgment v Γ idx ->
+  ⊢s Δ ->
+  (∀ x, (Γ d@ x).apply r.to = Δ d@ (r x)) ->
+  HsJudgment v Δ (idx_ren r idx)
+| .prf, (t, τ) , j, wf, f => match j with
+  | .implicitAllI h1 h2 => .implicitAllI sorry (rename r .prf h2 wf f)
+  | .implicitAllE h1 h2 => sorry
+  | .implicitArrI h1 h2 h3 => .implicitArrI (rename r .prf h1 wf f) sorry (rename r .prf h3 wf f)
+  | .implicitArrE h1 h2 => sorry
+  | .ax wf' => .ax wf
+  | .arrowk h1 h2 => .arrowk (rename r .prf h1 wf f) (rename r .prf h2 wf f)
+  | .appk h1 h2 =>
+    .appk (rename r .prf h1 wf f) (rename r .prf h2 wf f)
+  | @HsJudgment.allt Γ A _ h1 h2 =>
+      .allt (rename r .prf h1 wf f) sorry
+  | .arrow h1 h2  =>
+    .arrow (rename r .prf h1 wf f) sorry
+           -- (by have h' := rename r .prf h2 (.wfempty wf) (rename_lift r .empty f); rw[Subst.lift_lemma]; sorry)
+           -- (rename r .prf h2 (by sorry) (by sorry))
+
+  | @HsJudgment.var Γ x T wf' h => .var wf (by
+    have e := f x; unfold Frame.get_type at h;
+    split at h;
+    all_goals(cases h)
+    case _ h =>
+      have h' : (Γ d@ x).apply r.to = (Frame.kind T).apply r.to := by rw [h]
+      rw [e] at h'; unfold Frame.apply at h'; simp at h';
+      have h'' : (Δ d@ r x).get_type = (Frame.kind ([r.to] T)).get_type := by rw[h']
+      symm at h'';apply h'';
+    case _ h =>
+      have h' : (Γ d@ x).apply r.to = (Frame.type T).apply r.to := by rw [h]
+      rw [e] at h'; unfold Frame.apply at h'; simp at h';
+      have h'' : (Δ d@ r x).get_type = (Frame.type ([r.to] T)).get_type := by rw[h']
+      symm at h'';apply h'';
+    case _ => sorry
+    case _ => sorry
+    case _ => sorry
+    case _ => sorry
+    case _ => sorry
+    case _ => sorry)
+  | .lam h1 h2 h3 => .lam (rename r .prf h1 wf f) sorry (rename r .prf h3 wf f)
+  | .app h1 h2 h3 =>
+    .app (rename r .prf h1 wf f) (rename r .prf h2 wf f) (by rw [h3]; rw[<-Subst.lift_lemma]; sorry)
+  | .hslet h1 h2 h3 h4 =>
+    .hslet (rename r .prf h1 wf f) (rename r .prf h2 wf f) sorry (rename r .prf h4 wf f)
+  | .hsIte h1 h2 h3 h4 h5 h6 h7 h8 h9 h10 =>
+    .hsIte (rename r .prf h1 wf f) (rename r .prf h2 wf f) (rename r .prf h3 wf f) (rename r .prf h4 wf f)
+           (rename r .prf h5 wf f) (rename r .prf h6 wf f) sorry sorry (by sorry)  sorry
+| .wf, () , j, wf, r => by simp; apply wf
+
+
+def weaken :
+  ⊢s (f :: Γ) ->
+  Γ ⊢s t : A ->
+  (f::Γ) ⊢s ([S]t) : ([S]A)
+| wf , h => rename (λ x => x + 1) .prf h wf (by intro; rw [Subst.to_S]; simp)
+
+def weaken_empty :
+  Γ ⊢s t : A ->
+  (.empty::Γ) ⊢s ([S]t) : ([S]A)
+ := λ x => weaken (.wfempty (hs_judgment_ctx_wf .prf x)) x
+
+def weaken_type :
+  Γ ⊢s T : `★ ->
+  Γ ⊢s t : A ->
+  (.type T::Γ) ⊢s ([S]t) : ([S]A)
+:= λ h1 h2 => weaken (.wftype h1 (hs_judgment_ctx_wf .prf h1)) h2
+
+def weaken_kind :
+  Γ ⊢s T : `□ ->
+  Γ ⊢s t : A ->
+  (.kind T::Γ) ⊢s ([S]t) : ([S]A)
+:= sorry
+
+-- theorem weaken_kind :
+--   Γ ⊢s T : `□ ->
+--   Γ ⊢s t : A ->
+--   (.kind T::Γ) ⊢s ([S]t) : ([S]A)
+-- := by
+-- intro j1 j2; apply rename _ j2
+-- case _ => constructor; apply j1; apply hs_judgment_ctx_wf j1
+-- case _ => intro x; simp; rw [Subst.to_S]
+
+def weaken_datatype :
+  Γ ⊢s T : `□ ->
+  Γ ⊢s t : A ->
+  (.datatype T::Γ) ⊢s ([S]t) : ([S]A)
+:= sorry
+-- := by
+-- intro j1 j2; apply rename _ j2
+-- case _ => constructor; apply j1; apply hs_judgment_ctx_wf j1
+-- case _ => intro x; simp; rw [Subst.to_S]
+
+def weaken_ctor :
+  Γ ⊢s T : `★ ->
+  ValidHsCtorType Γ T ->
+  Γ ⊢s t : A ->
+  (.ctor T::Γ) ⊢s ([S]t) : ([S]A) := sorry
+-- := by
+-- intro j1 j2 j3; apply rename _ j3
+-- case _ => constructor; apply j1; apply hs_judgment_ctx_wf j1; apply j2
+-- case _ => intro x; simp; rw [Subst.to_S]
+
+def weaken_opent :
+  Γ ⊢s T : `□ ->
+  Γ ⊢s t : A ->
+  (.opent T::Γ) ⊢s ([S]t) : ([S]A) := sorry
+-- := by
+-- intro j1 j2; apply rename _ j2
+-- case _ => constructor; apply j1; apply hs_judgment_ctx_wf j1
+-- case _ => intro x; simp; rw [Subst.to_S]
+
+def weaken_openm :
+  Γ ⊢s T : `★ ->
+  Γ ⊢s t : A ->
+  (.openm T::Γ) ⊢s ([S]t) : ([S]A) := sorry
+-- by
+-- intro j1 j2; apply rename _ j2
+-- case _ => constructor; apply j1; apply hs_judgment_ctx_wf j1
+-- case _ => intro x; simp; rw [Subst.to_S]
+
+def weaken_insttype :
+  Γ ⊢s T : `★ ->
+  ValidHsInstType Γ T ->
+  Γ ⊢s t : A ->
+  (.insttype T::Γ) ⊢s ([S]t) : ([S]A) := sorry
+-- := by
+-- intro j1 j2 j3; apply rename _ j3
+-- case _ => constructor; apply j1; apply hs_judgment_ctx_wf j1; apply j2
+-- case _ => intro x; simp; rw [Subst.to_S]
+
+-- theorem weaken_inst :
+--   .openm T = Γ d@ x ->
+--   Γ ⊢s b : T ->
+--   Γ ⊢s t : A ->
+--   (.inst #x b::Γ) ⊢s ([S]t) : ([S]A)
+-- := by
+-- intro j1 j2 j3; apply rename _ j3
+-- case _ => constructor; apply j1; apply j2; apply hs_judgment_ctx_wf j2
+-- case _ => intro x; simp; rw [Subst.to_S]
+
+def weaken_term :
+  Γ ⊢s T : `★ ->
+  Γ ⊢s b : T ->
+  Γ ⊢s t : A ->
+  (.term T b::Γ) ⊢s ([S]t) : ([S]A)
+:= λ h1 h2 h3 => weaken (.wfterm h1 h2 (hs_judgment_ctx_wf .prf h1)) h3
